share/steel/examples/steel/dplex/out/EffectSystemProperties.ml
@@ -4,15 +4,14 @@ let pending (es : EffectStateMachine.effect_state) :
   (es.EffectStateMachine.client).MultiCollaboration.pending
 let pending_tail (es : EffectStateMachine.effect_state) :
   Domain.action Prims.list=
-  match pending es with | [] -> [] | uu___::tl -> tl
-let rec apply_events (next : Prims.nat -> Prims.nat)
-  (es : EffectStateMachine.effect_state)
+  match pending es with | [] -> [] | uu___::tl -> tl | uu___ -> []
+let rec apply_events (es : EffectStateMachine.effect_state)
   (events : EffectStateMachine.event Prims.list) :
   EffectStateMachine.effect_state=
   match events with
   | [] -> es
   | ev::tl ->
-      let uu___ = EffectStateMachine.step next es ev in
-      (match uu___ with | (es1, _cmd) -> apply_events next es1 tl)
+      let uu___ = EffectStateMachine.step es ev in
+      (match uu___ with | (es1, _cmd) -> apply_events es1 tl)
 type ('es, 'ev, 'a) processed_now = Obj.t
-type ('next, 'es, 'events, 'a) action_was_processed = Obj.t
+type ('es, 'events, 'a) action_was_processed = Obj.t
