share/steel/examples/steel/dplex/out/Selectors_Tree_Core.ml
@@ -1,0 +1,43 @@
+open Prims
+type 'a node =
+  {
+  data: 'a ;
+  left: 'a node Steel_Reference.ref ;
+  right: 'a node Steel_Reference.ref }
+let __proj__Mknode__item__data (projectee : 'a node) : 'a=
+  match projectee with | { data; left; right;_} -> data
+let __proj__Mknode__item__left (projectee : 'a node) :
+  'a node Steel_Reference.ref=
+  match projectee with | { data; left; right;_} -> left
+let __proj__Mknode__item__right (projectee : 'a node) :
+  'a node Steel_Reference.ref=
+  match projectee with | { data; left; right;_} -> right
+type 'a t = 'a node Steel_Reference.ref
+type 'a tree = 'a Trees.tree
+let get_left (n : 'a node) : 'a t= n.left
+let get_right (n : 'a node) : 'a t= n.right
+let get_data (n : 'a node) : 'a= n.data
+let mk_node (data : 'a) (left : 'a t) (right : 'a t) : 'a node=
+  { data; left; right }
+let null_t (uu___ : unit) : 'a t= Steel_Reference.null ()
+let is_null_t (ptr : 'a t) : Prims.bool= Steel_Reference.is_null ptr
+let rec tree_view : 'a . 'a node Trees.tree -> 'a Trees.tree =
+  fun tree1 ->
+    match tree1 with
+    | Trees.Leaf -> Trees.Leaf
+    | Trees.Node (data, left, right) ->
+        Trees.Node ((get_data data), (tree_view left), (tree_view right))
+
+
+
+let intro_linked_tree_leaf (uu___ : unit) : unit= ()
+let elim_linked_tree_leaf (ptr : 'a t) : unit= ()
+let node_is_not_null (ptr : 'a t) : unit= ()
+let pack_tree (ptr : 'a t) (left : 'a t) (right : 'a t) : unit= ()
+type ('a, 't1) is_node = Obj.t
+let reveal_non_empty_tree (ptr : 'a t) : unit= ()
+let unpack_tree_node (ptr : 'a t) : 'a node=
+  reveal_non_empty_tree ptr;
+  (let n = Steel_Reference.read ptr in Steel_Effect_Atomic.return () () n)
+let unpack_tree (ptr : 'a t) : 'a node=
+  let n = unpack_tree_node ptr in Steel_Effect_Atomic.return () () n
